% arara: indent: { cruft: /home/cmhughes/Desktop/tmp/, overwrite: on, trace: yes, silent: yes, onlyDefault: no}
some
other
text
\begin{enumerate}
	\item $3x^3y(-4x^3+y) = -12x^6y+3x^3y^2$
	\item $3x^3+y(-4x^3+y) = 3x^3-4x^3y+y^2$
	\item
	      \begin{align*}
	      	{\color{red}(3x^3+y)}(-4x^3+y) & =	{\color{red}(3x^3+y)}(-4x^3)+{\color{red}(3x^3+y)}(y) \\
	      	                               & =	-12x^6-4x^3y+3x^3y+y^2                                \\
	      	                               & =	-12x^6-x^3y+y^2
	      \end{align*}
\end{enumerate}
\begin{enumerate}
	\item $3x^3y(-4x^3+y) = -12x^6y+3x^3y^2$
	\item $3x^3+y(-4x^3+y) = 3x^3-4x^3y+y^2$
	\item
	      \begin{align*}
	      	{\color{red}(3x^3+y)}(-4x^3+y) & =	{\color{red}(3x^3+y)}(-4x^3)+{\color{red}(3x^3+y)}(y) \\
	      	                               & =	-12x^6-4x^3y+3x^3y+y^2                                \\
	      	                               & =	-12x^6-x^3y+y^2
	      \end{align*}
\end{enumerate}

\begin{something}
	\begin{else}
		again
	\end{else}
\end{something}
no
environments
here
\[ x^2+ 3x\]
other text
\[
	x^2+ 3x
\]
other text
